*** empty log message ***

examples/dev/AES/word8/word8CasesLib.sml
@@ -1,0 +1,127 @@
+(*===========================================================================*)
+(* Simple theory of bytes.                                                   *)
+(*===========================================================================*)
+
+(* Interactive mode:
+  load "word8Lib";
+  load "word8CasesTheory";
+*)
+structure word8CasesLib = struct
+open HolKernel Parse boolLib bossLib word8Lib word8Theory word8CasesTheory
+
+datatype clause = Var of term * term
+                | Num of int * term
+
+fun cvt_param (arg, res) =
+  if is_var arg then
+    Var (arg, res)
+  else if is_comb arg then
+    let val (n2w, nums) = strip_comb arg in
+      if term_eq ``n2w`` n2w andalso
+         length nums = 1 andalso
+         numSyntax.is_numeral (hd nums) then
+        Num (numSyntax.int_of_term (hd nums) mod 256, res)
+      else
+        raise (mk_HOL_ERR "word8Cases" "word8Define" 
+                          "bad syntax in word constant")
+    end
+  else
+    raise (mk_HOL_ERR "word8Cases" "word8Define"
+                      "argument must be a syntactic variable or word constant")
+
+fun to_first_var [] acc = (acc, NONE)
+  | to_first_var [Var x] acc = (acc, SOME x)
+  | to_first_var [Num x] acc = (x :: acc, NONE)
+  | to_first_var (Var x :: t) acc = 
+      (HOL_WARNING "word8Cases" "word8Define"
+                   "ignoring cases after variable parameter case";
+       (rev acc, SOME x))
+  | to_first_var (Num x :: t) acc = 
+      to_first_var t (x :: acc)
+
+fun fill_results_helper next i j r default warn = 
+  let val first_pad_amt  = i - next 
+      val second_pad_amt = j - i - 1
+  in
+    if first_pad_amt > 0 orelse second_pad_amt > 0 then
+      warn ()
+    else ();
+    (List.tabulate (first_pad_amt, default) @ [r] @
+      List.tabulate (second_pad_amt, default),
+     next + 1 + first_pad_amt + second_pad_amt)
+  end
+
+fun fill_results [] default warn next =
+      if next = 256 then
+        []
+      else
+       (warn ();
+        List.tabulate (256 - next, default))
+  | fill_results [(i, r)] default warn next =
+      #1 (fill_results_helper next i 256 r default warn)
+  | fill_results ((i, r1) :: (j, r2) :: t) default warn next = 
+      if i = j then
+        raise (mk_HOL_ERR "word8Cases" "word8Define"
+                        ("duplicate definitions for " ^ int_to_string i ^ "w"))
+      else 
+        let val (rs, next_next) = 
+                fill_results_helper next i j r1 default warn
+        in 
+          rs @ fill_results ((j, r2) :: t) default warn next_next
+        end
+
+fun word8Define def_term = 
+  let val clauses = strip_conj def_term
+      val name = #1 (strip_comb (#1 (dest_eq (hd clauses))))
+      val params = map (hd o #2 o strip_comb o #1 o dest_eq) clauses
+      val results = map (#2 o dest_eq) clauses
+      val (num_params, var_param) =
+        to_first_var (map cvt_param (zip params results)) []
+      val s_num_params = sort (fn (x, _) => fn (y, _) => x < y) num_params
+      val result_type = type_of (hd results)
+      val results_no_gaps = 
+        fill_results s_num_params
+                     (case var_param of
+                        SOME (var, res) => (fn _ => res)
+                      | NONE => 
+                         (fn _ => mk_arb result_type))
+                     (case var_param of
+                        SOME (var, res) => (fn _ => ())
+                      | NONE => (fn _ =>
+                                  HOL_WARNING "word8Cases" "word8Definition"
+                                              "cases not exhaustive"))
+                     0
+      val def = Define 
+      `^name = ^(list_mk_comb (inst [alpha |-> result_type] ``word8_cases``, 
+                               results_no_gaps))`
+      val simp_def = WORD_RULE (PURE_ONCE_REWRITE_RULE [word8_cases_def] def)
+      val eqns =
+        (map (fn (num, res) =>
+                ``^(#1 (dest_eq (concl def)))
+                  (n2w ^(numSyntax.term_of_int num)) =
+                  ^res``)
+              s_num_params) @
+        (case var_param of
+           SOME (var, res) => [``!^var. ^name ^var = ^res``]
+         | NONE => [])
+      val thms =
+        map (fn e => prove (e, PURE_ONCE_REWRITE_TAC [simp_def] THEN WORD_TAC))
+            eqns
+  in
+    (def, simp_def, LIST_CONJ thms)
+  end
+
+
+end
+(*
+word8Define ``f (x:word8) = 1``;
+word8Define ``f (x:word8) = x``;
+word8Define ``f 1w = 1``;
+word8Define ``(f 1w = 1) /\ (f x = 2)``;
+word8Define ``(f 0w = 1) /\ (f x = 2) /\ (f 0w = 3)``;
+word8Define ``(f 0w = 1) /\ (f 2w = 2) /\ (f 4w = 3)``;
+word8Define ``(f 1w = 1) /\ (f 3w = 2) /\ (f 5w = 3)``;
+word8Define ``(f 0w = 1) /\ (f 256w = 1)`` handle e => Raise e;
+word8Define ``(f 0 = 1)`` handle e => Raise e;
+word8Define ``(f (a b) = 1)`` handle e => Raise e;
+*)
