examples/dev/AES/word8/word8CasesScript.sml
@@ -3,22 +3,16 @@
 (*===========================================================================*)
 
 (* Interactive mode:
-  load "word8Lib";
-*)
+  load "word8Lib";*)
+
 open HolKernel Parse boolLib bossLib word8Lib word8Theory
 
 val _ = new_theory "word8Cases"
 
 fun buildVar name t n = mk_var ((name ^ int_to_string n), t)
-
-val word8Type = mk_type ("word8", [])
-val alphaType = mk_vartype "'a"
 val nums = upto 0 255
-val vars = map (buildVar "w" alphaType) nums
+val vars = map (buildVar "w" alpha) nums
 val consts = map (fn n => ``n2w ^(numSyntax.term_of_int n)``) nums
-
-
-local
 
 val bound_thm = Q.prove (
 `!x. ?y. y < 256 /\ (x = n2w y)`,
@@ -30,14 +24,10 @@ val lem = Q.prove (
  `!c.(0 < c /\ P (c - 1) /\ !n. n < c - 1 ==> P n) ==>(!n. n < c ==> P n)`,
 RW_TAC arith_ss [arithmeticTheory.BOUNDED_FORALL_THM]);
 
-in
-
 fun CASES256 w x =
 `?n. n < 256 /\ (^w = n2w n)` by RW_TAC std_ss [bound_thm] THEN
 RW_TAC std_ss [] THEN (POP_ASSUM MP_TAC) THEN
 Q.SPEC_TAC (`n`, `n`) THEN REPEAT (HO_MATCH_MP_TAC lem THEN x)
-
-end
 
 val nchotomy = Q.prove (
 `!x. ^(list_mk_disj (map (fn c => ``x = ^c``) (rev consts)))`,
@@ -49,58 +39,24 @@ STRIP_TAC THEN CASES256 ``x:word8``
                    Q.SPEC_TAC (`n`, `n`)]) THEN
 Cases THEN RW_TAC arith_ss [])
 
-local
+val _ = save_thm ("word8Nchotomy", nchotomy);
 
-val i_t = numSyntax.term_of_int
-
-val pr_body_eqns = map2 (fn c => fn v => ``fn ^c = ^v``) 
-                        consts vars
-fun mk_witness low hi = 
+fun mk_body low hi var results = 
   if low = hi then
-    List.nth (vars, low)
+    List.nth (results, low)
   else
     let val mid = (hi + low) div 2 in
-      mk_cond (``w2n x <= ^(i_t mid)``,
-               mk_witness low mid,
-               mk_witness (mid + 1) hi)
+      mk_cond (``w2n ^var <= ^(numSyntax.term_of_int mid)``,
+               mk_body low mid var results,
+               mk_body (mid + 1) hi var results)
     end
-val pr_witness = ``\x. ^(mk_witness 0 255)``
 
-val use_top_assum = POP_ASSUM (fn thm => PURE_ONCE_REWRITE_TAC [GSYM thm])
-
-val prim_rec = prove (
-list_mk_forall (vars, ``?!fn. (\fn. ^(list_mk_conj pr_body_eqns)) fn``),
-REPEAT GEN_TAC THEN REWRITE_TAC [EXISTS_UNIQUE_THM] THEN BETA_TAC THEN
-REPEAT STRIP_TAC
-THENL
- [EXISTS_TAC pr_witness THEN REPEAT STRIP_TAC THEN BETA_TAC THEN WORD_TAC,
-  ALL_TAC] THEN
-NTAC 256 (POP_ASSUM MP_TAC) THEN
-NTAC 256 use_top_assum THEN
-REPEAT STRIP_TAC THEN
-CONV_TAC FUN_EQ_CONV THEN GEN_TAC THEN
-CASES256 ``w:word8`` (SIMP_TAC arith_ss [] THEN CONJ_TAC THENL
-              [POP_ASSUM (ACCEPT_TAC o GSYM), POP_ASSUM (K ALL_TAC)]) THEN
-Cases_on `n` THEN RW_TAC arith_ss [])
-in 
+val body = mk_body 0 255 ``x:word8`` vars
 
 val word8_cases_def = Define
-`word8_cases = ^(list_mk_abs (vars, pr_witness))`
+`word8_cases = ^(list_mk_abs (vars, ``\x.^body``))`;
 
-val word8UniquePrimRec = BETA_RULE prim_rec
-
-val word8PrimRec = 
-GENL vars
- (BETA_RULE (hd (BODY_CONJUNCTS (REWRITE_RULE [EXISTS_UNIQUE_THM] prim_rec))))
-
-val induct = Prim_rec.prove_induction_thm word8UniquePrimRec
-
-end
-
-
-
-local 
-
+(*
 val f = #1 (dest_eq (concl word8_cases_def));
 val clauses =
   map2 (fn c => fn v =>
@@ -112,41 +68,45 @@ val thms =
          prove (clause, PURE_ONCE_REWRITE_TAC [word8_cases_def] THEN WORD_TAC))
       clauses
 
-in
-val cases = GENL vars (LIST_CONJ thms)
+val cases = LIST_CONJ thms
 
-end
-
-val _ = save_thm("word8Nchotomy", nchotomy)
-val _ = save_thm("word8UniquePrimRec",word8UniquePrimRec)
-val _ = save_thm("word8PrimRec",word8PrimRec)
-val _ = save_thm("word8Induct",induct)
-val _ = save_thm("word8Cases", cases)
-
-
-(*
-local
-
-fun fold_term f [x] = x
-  | fold_term f (h::t) = f (h, (fold_term f t))
-
-val less_than_lems =
-  map (fn n => prove (``^(numSyntax.term_of_int n) < 256``,
-                      RW_TAC list_ss [])) nums
-
-val not_eq_thms = flatten
-  (List.map (fn i =>
-              List.map (fn j =>
-                          Q.prove (`~(n2w ^(numSyntax.term_of_int i) =
-                                   n2w ^(numSyntax.term_of_int j))`,
-                                 SIMP_TAC arith_ss [not_eq_lem]))
-                       (upto 0 (i - 1)))
-            nums)
-
-in
-val distinct = LIST_CONJ not_eq_thms
-end
-
+val _ = save_thm("word8Cases", cases);
 *)
-val _ = export_theory();
 
+val pr_body_eqns = map2 (fn c => fn v => ``fn ^c = ^v``) 
+                        consts vars
+
+val use_top_assum = POP_ASSUM (fn thm => PURE_ONCE_REWRITE_TAC [GSYM thm])
+
+val witness =
+ snd (dest_eq (concl (BETA_RULE (PURE_ONCE_REWRITE_CONV [word8_cases_def]
+                                  (list_mk_comb (``word8_cases``, vars))))))
+
+val prim_rec = prove (
+list_mk_forall (vars, ``?!fn. (\fn. ^(list_mk_conj pr_body_eqns)) fn``),
+REPEAT GEN_TAC THEN PURE_ONCE_REWRITE_TAC [EXISTS_UNIQUE_THM] THEN
+BETA_TAC THEN REPEAT STRIP_TAC
+THENL
+ [EXISTS_TAC witness THEN REPEAT STRIP_TAC THEN WORD_TAC,
+  ALL_TAC] THEN
+NTAC 256 (POP_ASSUM MP_TAC) THEN
+NTAC 256 use_top_assum THEN
+REPEAT STRIP_TAC THEN
+CONV_TAC FUN_EQ_CONV THEN GEN_TAC THEN
+CASES256 ``w:word8`` (SIMP_TAC arith_ss [] THEN CONJ_TAC THENL
+              [POP_ASSUM (ACCEPT_TAC o GSYM), POP_ASSUM (K ALL_TAC)]) THEN
+Cases_on `n` THEN RW_TAC arith_ss [])
+
+val word8UniquePrimRec = BETA_RULE prim_rec
+
+val word8PrimRec = 
+GENL vars
+ (BETA_RULE (hd (BODY_CONJUNCTS (REWRITE_RULE [EXISTS_UNIQUE_THM] prim_rec))))
+
+val induct = Prim_rec.prove_induction_thm word8UniquePrimRec
+
+val _ = save_thm ("word8PrimRec", word8PrimRec)
+val _ = save_thm ("word8UniquePrimRec", word8UniquePrimRec)
+val _ = save_thm ("word8Induct", induct);
+
+val _ = export_theory();
